Risc0/State/Update.lean
@@ -23,13 +23,25 @@ namespace Risc0.State
     update state name (.some (.Constraint c)) = { state with props := state.props.update ⟨name⟩ c } := rfl
 
   @[simp]
-  lemma update_skip_felts (h: name' ≠ name) :
-    (State.felts (update st name' x) { name }) = (State.felts st { name }) := by
-      simp only [State.update]
-      aesop'
+  private lemma updateMany_consecutiveUpdates_of_ne {m : Map FeltVar Felt}
+    (h : ¬isSpecial name') :
+    (m.updateMany (consecutiveUpdates name l)) (⟨name'⟩ : FeltVar) = m (⟨name'⟩ : FeltVar) := by
+    simp [consecutiveUpdates]
+    generalize 0 = k
+    induction l generalizing k with
+      | nil => simp
+      | cons hd tl ih => simp; rw [Map.update_get_next', ih]; simp
+                         rintro ⟨contra⟩
+                         exact absurd (isSpecial_toString_SpecialSymbol_app) h
 
   @[simp]
-  lemma update_skip_nested_felts (h: name' ≠ name) :
+  lemma update_skip_felts (h: name' ≠ name) (h' : ¬isSpecial name):
+    (State.felts (update st name' x) { name }) = (State.felts st { name }) := by
+      simp only [State.update]
+      aesop
+
+  @[simp]
+  lemma update_skip_nested_felts (h: name' ≠ name) (h' : ¬isSpecial name):
     (State.felts (update ( update st name' x) name y) { name }) = (State.felts (update st name y) { name }) := by
     simp [h, State.update]
     aesop'
